Makefile
@@ -97,7 +97,7 @@ BACKEND=\
   Bounds.v Stacklayout.v Stacking.v Stackingproof.v \
   Machblock.v Machblockgen.v Machblockgenproof.v \
   Asmblock.v Asmblockgen.v Asmblockgenproof.v \
-  Asm.v Asmgen.v Asmgenproof0.v Asmgenproof1.v Asmgenproof.v
+  Asm.v Asmgen.v Asmgenproof.v
 
 # C front-end modules (in cfrontend/)
 
